Adjoin operation on traces  (#126)
adjoin definition & trace construction

* rename trace_seq --> traceSeq

* a note on partial monoid instance for traces

Unfortunately, it is impossible to declare an instance of partial monoid for traces (in the current formulation).
In order to do that we need to embed an absorbing element into trace type, but then we will lose `subType` injection to `seq`, we will have to perform case-analysis everywhere, and we will face other obstacles.
Thus, a better solution would be to give up on monoid instance for traces, and declare it (later) only for trace languages.

theories/concur/lts.v
@@ -21,6 +21,8 @@ From eventstruct Require Import utils relalg.
 (*                      from s1 to s2.                                        *)
 (*            step S == a type of steps of the LTS.                           *)
 (*                   := { (lbl, src, dst) | src --[lbl]--> dst }.             *)
+(*         step_of H == given a proof of step property H : s --[l]--> s'      *)
+(*                      constructs a step { (l, s, s') | s --[l]--> s' }.     *)
 (*           trace S == a type of traces of the LTS, that is finite sequences *)
 (*                      of steps performed by the transition system.          *)
 (*                   := { tr : seq (step S) | dst tr[i] == src tr[i+1] }.     *)
@@ -28,10 +30,16 @@ From eventstruct Require Import utils relalg.
 (*                      Coq must be able to infer a proof that ts satisfies   *)
 (*                      trace property (i.e the ends of steps should match).  *)
 (*           [trace] == empty trace.                                          *)
-(*         labels tr == a sequence of labels of tr.                           *)
-(*       states s tr == a sequence of states of tr or [:: s] is tr is empty.  *)
-(*    fst_state s tr == the first state of of tr or s is tr is empty.         *)
-(*    lst_state s tr == the last state of of tr or s is tr is empty.          *)
+(*       tr1 <+> tr2 == concatenation of traces tr1 ++ tr2 if tr1 and tr2     *)
+(*                      are adjoint, empty trace otherwise.                   *)
+(*          st <+ tr == cons of step st and trace tr if they are are adjoint, *)
+(*                      empty trace otherwise.                                *)
+(*          tr +> st == rcons of step st and trace tr if they are are adjoint,*)
+(*                      empty trace otherwise.                                *)
+(*         labels tr == a sequence of labels of a trace.                      *)
+(*       states s tr == a sequence of states of tr or [:: s] if tr is empty.  *)
+(*    fst_state s tr == the first state of tr or s is tr is empty.            *)
+(*    lst_state s tr == the last state of tr or s is tr is empty.             *)
 (*   adjoint tr1 tr2 == a relation asserting that two traces are adjoint,     *)
 (*                      meaning that the last state of tr1 is equal to        *)
 (*                      the first state of tr2.                               *)
@@ -159,23 +167,28 @@ Module Export Step.
 
 Section Def.
 Context {L : Type} (S : ltsType L).
+Implicit Types (l : L) (s : S).
 
 Record stepTuple : Type := mk_step {
   lbl : L; src : S; dst : S;  
 }.
 
 Definition is_step : pred stepTuple := 
-  fun s => (src s) --[lbl s]--> (dst s).
+  fun st => (src st) --[lbl st]--> (dst st).
 
 Structure step : Type := Step {step_val :> stepTuple; _ : is_step step_val}.
 
 Canonical step_subType := Eval hnf in [subType for step_val].
 
+Definition step_of l s s' : (s --[l]--> s') -> step := 
+  fun p => @Step (mk_step l s s') p.
+
 Definition adj : rel step := 
-  fun s t => dst s == src t. 
+  fun st st' => dst st == src st'. 
+
 End Def.
 
-Prenex Implicits lbl src dst is_step adj.
+Prenex Implicits lbl src dst is_step step_of adj.
 
 Section EQ. 
 Context {L : eqType} (S : ltsType L).
@@ -201,41 +214,52 @@ Canonical step_eqType := Eval hnf in EqType (step S) step_eqMixin.
 
 End EQ.
 
+Section Theory.
+Context {L : eqType} (S : ltsType L).
+Implicit Types (l : L) (s : S).
+
+Lemma step_of_val l s s' (Hst : s --[l]--> s') : 
+  step_of Hst = mk_step l s s' :> stepTuple S.
+Proof. done. Qed.
+
+End Theory.
+
 End Step.
 
 
 Module Export Trace. 
 
-Notation trace_seq S := (seq (step S)).
+Notation traceSeq S := (seq (step S)).
 
 Section Def. 
 Context {L : Type} (S : ltsType L).
 
-Definition is_trace : pred (trace_seq S) := 
+Definition is_trace : pred (traceSeq S) := 
   fun ts => sorted adj ts.
 
 Structure trace : Type := Trace { 
-  trace_val :> trace_seq S; 
+  trace_val :> traceSeq S; 
   _         :  is_trace trace_val;
 }.
 
 Canonical trace_subType := Eval hnf in [subType for trace_val].
 
-Implicit Types (ts : trace_seq S) (tr : trace).
+Implicit Types (ts : traceSeq S) (tr : trace).
 
-Definition labels : trace_seq S -> seq L := map (lbl : step S -> L). 
+Definition labels : traceSeq S -> seq L := map (lbl : step S -> L). 
 
-Definition states : S -> trace_seq S -> seq S := 
+Definition states : S -> traceSeq S -> seq S := 
   fun s ts => 
     match ts with 
     | [::]    => [:: s] 
     | st :: _ => src st :: map (dst : step S -> S) ts
     end. 
 
-Definition fst_state : S -> trace_seq S -> S := 
+(* TODO: try `starts_with` and `ends_with` predicates instead? *)
+Definition fst_state : S -> traceSeq S -> S := 
   fun s ts => if ts is st :: ts then src st else s.
 
-Definition lst_state : S -> trace_seq S -> S := 
+Definition lst_state : S -> traceSeq S -> S := 
   fun s ts => if ts is st :: ts then dst (last st ts) else s. 
 
 Definition trace_lang : S -> pred trace := 
@@ -245,12 +269,15 @@ Definition trace_lang : S -> pred trace :=
 Definition lts_lang : S -> lang L := 
   fun s w => exists2 tr, trace_lang s tr & w = labels tr.
 
-Definition adjoint : rel (trace_seq S) := 
+Definition adjoint : rel (traceSeq S) := 
   fun ts1 ts2 => 
     match ts2 with 
     | [::]    => true
     | st :: _ => lst_state (src st) ts1 == src st
     end.
+
+Definition adjoin : traceSeq S -> traceSeq S -> traceSeq S :=
+  fun ts1 ts2 => if adjoint ts1 ts2 then ts1 ++ ts2 else [::].
 
 Definition mk_trace tr mkTr : trace :=
   mkTr (let: Trace _ trP := tr return is_trace tr in trP).
@@ -259,21 +286,57 @@ End Def.
 
 Arguments adjoint : simpl never.
 
-Section Seq.
-Context {L : Type} (S : ltsType L).
-Implicit Types (st : step S) (s : trace_seq S) (tr : trace S).
-
-Lemma nil_traceP : is_trace ([::] : seq (step S)).
-Proof. done. Qed.
-Canonical nil_trace := Trace nil_traceP.
-
-End Seq.
-
 Notation "[ 'trace' 'of' tr ]" := (mk_trace (fun trP => @Trace _ _ tr trP))
   (at level 0, format "[ 'trace'  'of'  tr ]") : form_scope.
 
 Notation "[ 'trace' ]" := [trace of [::]]
   (at level 0, format "[ 'trace' ]") : form_scope.
+
+Notation "tr1 '<+>' tr2" := [trace of adjoin tr1 tr2]
+  (at level 51, left associativity) : lts_scope.
+
+Notation "st '<+' tr" := [trace of adjoin [:: st] tr]
+  (at level 49, right associativity) : lts_scope.
+
+Notation "tr '+>' st" := [trace of adjoin tr [:: st]]
+  (at level 48, left associativity) : lts_scope.
+
+
+Section Build.
+Context {L : Type} (S : ltsType L).
+Implicit Types (st : step S) (ts : traceSeq S) (tr : trace S).
+
+Lemma nil_traceP : is_trace ([::] : seq (step S)).
+Proof. done. Qed.
+Canonical nil_trace := Trace nil_traceP.
+
+Lemma singl_traceP st : is_trace [:: st].
+Proof. done. Qed.
+Canonical singl_trace st := Trace (singl_traceP st).
+
+Lemma adjoin_traceP tr1 tr2 : is_trace (adjoin tr1 tr2).
+Proof. 
+  case: tr1=> [ts1]; case: tr2=> [ts2] /=.
+  rewrite /adjoin /is_trace. 
+  case: ifP=> [|?] //.
+  case: ts1=> [|st1 {}ts1] //=; rewrite cat_path.
+  case: ts2=> [|st2 {}ts2] //= ???; [exact/andP | exact/and3P].
+Qed.
+Canonical adjoin_trace tr1 tr2 := Trace (adjoin_traceP tr1 tr2).
+
+Lemma adjoin_val tr1 tr2 : 
+  adjoint tr1 tr2 -> tr1 <+> tr2 = tr1 ++ tr2 :> traceSeq S.
+Proof. by rewrite /adjoin /=; case: ifP. Qed.
+
+Lemma adjoin_cons_val st tr : 
+  adjoint [:: st] tr -> st <+ tr = st :: tr :> traceSeq S.
+Proof. by rewrite /adjoin /=; case: ifP. Qed.
+
+Lemma adjoin_rcons_val st tr : 
+  adjoint tr [:: st] -> tr +> st = rcons tr st :> traceSeq S.
+Proof. by rewrite /adjoin -cats1 /=; case: ifP. Qed.
+
+End Build.
 
 Section EQ.
 Context {L : eqType} (S : ltsType L).
@@ -285,7 +348,7 @@ End EQ.
 
 Section Theory. 
 Context {L : Type} (S : ltsType L).
-Implicit Types (st : step S) (ts : trace_seq S) (tr : trace S).
+Implicit Types (st : step S) (ts : traceSeq S) (tr : trace S).
 
 Lemma trace_adj tr : sorted adj tr.
 Proof. by case: tr. Qed.
@@ -378,7 +441,8 @@ Lemma labels_cat ts1 ts2 :
   labels (ts1 ++ ts2) = labels ts1 ++ labels ts2.
 Proof. by rewrite /labels map_cat. Qed.
 
-Lemma size_states s ts : size (states s ts) == (size ts).+1.
+Lemma size_states s ts : 
+  size (states s ts) == (size ts).+1.
 Proof. by rewrite /states; case: ts=> [|??] //=; rewrite size_map. Qed.
                          
 Lemma states_rcons s ts st : s = fst_state (src st) ts -> 
@@ -388,6 +452,14 @@ Proof. by case: ts=> [->|??] //=; rewrite map_rcons. Qed.
 Lemma states_cat s ts1 ts2 : s = fst_state s ts2 -> 
   states s (ts1 ++ ts2) = states s ts1 ++ behead (states s ts2).
 Proof. by rewrite /states map_cat; case: ts1; case: ts2=> //= ?? ->. Qed.
+
+Lemma adjoin0s tr : 
+  [trace] <+> tr = tr.
+Proof. by apply/val_inj=> /=; rewrite adjoin_val ?adjoint0s //=. Qed.  
+
+Lemma adjoins0 tr : 
+  tr <+> [trace] = tr.
+Proof. by apply/val_inj=> /=; rewrite adjoin_val ?adjoints0 ?cats0 //=. Qed.
 
 End Theory.
 
@@ -472,15 +544,8 @@ Proof.
   case: (nilp tr)/nilP=> [->|Hnil] /=. 
   - move: (valP st); rewrite /is_step=> /[swap] <- => Hs. 
     move: (sim_step HR Hs)=> [s' HR' Hs'].
-    (* TODO: introduce a nicer way to construct steps 
-     *   (using canonical structures and phantom types?) 
-     *)
-    pose st_' := mk_step (lbl st) s s'. 
-    have Hst' : is_step st_' by done. 
-    pose st'  := Step Hst'.     
-    have Htr' : is_trace [:: st']. 
-    - by rewrite is_trace_cons //=; apply/andP.
-    by exists (Trace Htr')=> //=. 
+    pose st' := step_of Hs'. 
+    by exists [trace of [:: st']]. 
   rewrite (fst_stateNnil t) // => Ht.
   move: (IH Htr Ht); clear IH. 
   move=> [tr' []] /[swap].
@@ -494,15 +559,10 @@ Proof.
   - rewrite /nilp -size_labels -Hlbl size_labels. 
     by move: Hnil=> /nilP.
   move=> /nilP Hnil'.
-  pose st_' := mk_step (lbl st) (lst_state s tr') s'.
-  have Hst' : is_step st_' by done.
-  pose st'  := Step Hst'.
-  have Htr' : is_trace (rcons tr' st'). 
-  - rewrite is_trace_rcons; apply /andP; split=> //.
-    - exact/(valP tr').
-    rewrite adjoint_lastE /=.
-    by apply/eqP/lst_stateNnil.
-  exists (Trace Htr')=> /=; split.
+  pose st' := step_of Hs'.
+  exists (tr' +> st')=> /=.
+  rewrite !adjoin_rcons_val; last first; [|split].
+  - by rewrite /adjoint step_of_val (lst_stateNnil s) /=. 
   - by rewrite !lst_state_rcons /=.
   - by rewrite labels_rcons Hlbl.
   rewrite fst_state_rcons Hfst -fst_state_src. 
